Source/DafnyCore/AST/Modules/LiteralModuleDecl.cs
@@ -46,8 +46,9 @@ public class LiteralModuleDecl : ModuleDecl, ICanFormat, IHasSymbolChildren {
   }
 
   [SyntaxConstructor]
-  public LiteralModuleDecl(DafnyOptions options, IOrigin origin, Name nameNode, Attributes? attributes, ModuleDefinition enclosingModule, string cloneId, ModuleDefinition moduleDef)
-    : base(options, origin, nameNode, attributes, enclosingModule, cloneId) {
+  public LiteralModuleDecl(DafnyOptions options, IOrigin origin, Name nameNode, Attributes? attributes, 
+    ModuleDefinition enclosingModuleDefinition, string cloneId, ModuleDefinition moduleDef)
+    : base(options, origin, nameNode, attributes, enclosingModuleDefinition, cloneId) {
     ModuleDef = moduleDef;
     BodyStartTok = moduleDef.BodyStartTok;
     moduleDef.EnclosingLiteralModuleDecl = this;
