Source/DafnyCore/AST/TypeDeclarations/ClassLikeDecl.cs
@@ -26,12 +26,12 @@ public abstract class ClassLikeDecl : TopLevelDeclWithMembers, RevealableTypeDec
 
   [SyntaxConstructor]
   protected ClassLikeDecl(IOrigin origin, Name nameNode, Attributes attributes,
-    List<TypeParameter> typeArgs, ModuleDefinition enclosingModule,
+    List<TypeParameter> typeArgs, ModuleDefinition enclosingModuleDefinition,
     [Captured] List<MemberDecl> members, List<Type> traits /*?*/)
-    : base(origin, nameNode, enclosingModule, typeArgs, members, attributes, traits) {
+    : base(origin, nameNode, enclosingModuleDefinition, typeArgs, members, attributes, traits) {
     Contract.Requires(origin != null);
     Contract.Requires(nameNode != null);
-    Contract.Requires(enclosingModule != null);
+    Contract.Requires(enclosingModuleDefinition != null);
     Contract.Requires(cce.NonNullElements(typeArgs));
     Contract.Requires(cce.NonNullElements(members));
   }
