Source/IntegrationTests/TestFiles/LitTests/LitTest/cli/inputFormat.dfy
@@ -2,6 +2,59 @@
 // RUN: ! %verify --input-format Binary --stdin < %t.assertFalse.dbin > %t
 // RUN: %diff "%s.expect" "%t"
 
-method Foo() {
-  assert false;
+// additional.dfy
+
+const intMax := 4294967296
+
+type nat32 = x: int32
+  | x >= 0
+
+type int32 = x: int
+  | -4294967296 < x && x < intMax
+
+class Fibonacci {
+  static function Spec(n: nat): nat
+  {
+    if n < 2 then
+      n
+    else
+      Spec(n - 1) + Spec(n - 2)
+  }
+
+  static method Implementation(n: nat32) returns (r: nat32)
+    requires Spec(n) <= 2147483647
+    ensures r == Spec(n)
+  {
+    if n == 0 {
+      return 0;
+    }
+    var previousResult: int32 := 0;
+    var result: int32 := 1;
+    var i: int32 := 1;
+    while i < n
+      invariant result == Spec(i)
+      invariant previousResult == Spec(i - 1)
+      invariant i <= n
+    {
+      i := i + 1;
+      SpecIsIncreasing(i, n);
+      var addition: int32 := result + previousResult;
+      previousResult := result;
+      result := addition;
+    }
+    return result;
+  }
+
+  static method SpecIsIncreasing(i: nat, j: nat)
+    requires i <= j
+    ensures Spec(i) <= Spec(j)
+  {
+    var x := i;
+    while(x < j) 
+      invariant x <= j
+      invariant Spec(i) <= Spec(x)
+    {
+      x := x + 1;
+    }
+  }
 }
